<?xml version="1.0"?>
<rdf:RDF xmlns="http://emmo.info/emmo/middle/metrology#"
     xml:base="http://emmo.info/emmo/middle/metrology"
     xmlns:owl="http://www.w3.org/2002/07/owl#"
     xmlns:rdf="http://www.w3.org/1999/02/22-rdf-syntax-ns#"
     xmlns:xml="http://www.w3.org/XML/1998/namespace"
     xmlns:xsd="http://www.w3.org/2001/XMLSchema#"
     xmlns:rdfs="http://www.w3.org/2000/01/rdf-schema#"
     xmlns:skos="http://www.w3.org/2004/02/skos/core#"
     xmlns:dcterms="http://purl.org/dc/terms/"
     xmlns:annotations="http://emmo.info/emmo/top/annotations#">
    <owl:Ontology rdf:about="http://emmo.info/emmo/middle/metrology">
        <owl:versionIRI rdf:resource="http://emmo.info/emmo/1.0.0-alpha2/middle/metrology"/>
        <owl:imports rdf:resource="http://emmo.info/emmo/1.0.0-alpha2/middle/math"/>
        <owl:imports rdf:resource="http://emmo.info/emmo/1.0.0-alpha2/middle/perceptual"/>
        <owl:imports rdf:resource="http://emmo.info/emmo/1.0.0-alpha2/middle/physicalistic"/>
        <owl:imports rdf:resource="http://emmo.info/emmo/1.0.0-alpha2/middle/properties"/>
        <dcterms:abstract xml:lang="en">European Materials &amp; Modelling Ontology (EMMO)

EMMO is a multidisciplinary effort to develop a standard representational framework (the ontology) based on current materials modelling knowledge, including physical sciences, analytical philosophy and information and communication technologies.

It provides the connection between the physical world, materials characterisation world and materials modelling world.

EMMO is released under a Creative Commons license Attribution 4.0 International (CC BY 4.0).</dcterms:abstract>
        <dcterms:contributor>Access, DE</dcterms:contributor>
        <dcterms:contributor>Fraunhofer IWM, DE</dcterms:contributor>
        <dcterms:contributor>Goldbeck Consulting Ltd (UK)</dcterms:contributor>
        <dcterms:contributor>SINTEF, NO</dcterms:contributor>
        <dcterms:contributor>University of Bologna, IT</dcterms:contributor>
        <dcterms:creator>Adham Hashibon</dcterms:creator>
        <dcterms:creator>Emanuele Ghedini</dcterms:creator>
        <dcterms:creator>Georg Schmitz</dcterms:creator>
        <dcterms:creator>Gerhard Goldbeck</dcterms:creator>
        <dcterms:creator>Jesper Friis</dcterms:creator>
        <dcterms:license>https://creativecommons.org/licenses/by/4.0/legalcode</dcterms:license>
        <dcterms:publisher>EMMC ASBL</dcterms:publisher>
        <dcterms:title xml:lang="en">European Materials &amp; Modelling Ontology</dcterms:title>
        <rdfs:comment xml:lang="en">Contacts:
Gerhard Goldbeck
Goldbeck Consulting Ltd (UK)
email: gerhard@goldbeck-consulting.com

Emanuele Ghedini
University of Bologna (IT)
email: emanuele.ghedini@unibo.it</rdfs:comment>
        <rdfs:comment xml:lang="en">The EMMO requires FacT++ reasoner plugin in order to visualize all inferences and class hierarchy (ctrl+R hotkey in Protege).</rdfs:comment>
        <owl:versionInfo>1.0.0-alpha2</owl:versionInfo>
    </owl:Ontology>
    


    <!-- 
    ///////////////////////////////////////////////////////////////////////////////////////
    //
    // Object Properties
    //
    ///////////////////////////////////////////////////////////////////////////////////////
     -->

    


    <!-- http://emmo.info/emmo/middle/metrology#EMMO_67fc0a36_8dcb_4ffa_9a43_31074efa3296 -->

    <owl:ObjectProperty rdf:about="http://emmo.info/emmo/middle/metrology#EMMO_67fc0a36_8dcb_4ffa_9a43_31074efa3296">
        <rdfs:subPropertyOf rdf:resource="http://emmo.info/emmo/middle/reductionistic#EMMO_b2282816_b7a3_44c6_b2cb_3feff1ceb7fe"/>
        <rdf:type rdf:resource="http://www.w3.org/2002/07/owl#InverseFunctionalProperty"/>
        <rdf:type rdf:resource="http://www.w3.org/2002/07/owl#AsymmetricProperty"/>
        <rdf:type rdf:resource="http://www.w3.org/2002/07/owl#IrreflexiveProperty"/>
        <rdfs:domain rdf:resource="http://emmo.info/emmo/middle/metrology#EMMO_f658c301_ce93_46cf_9639_4eace2c5d1d5"/>
        <rdfs:range rdf:resource="http://emmo.info/emmo/middle/metrology#EMMO_18ce5200_00f5_45bb_8c6f_6fb128cd41ae"/>
        <rdfs:comment xml:lang="en">Relates the physical quantity to its unit through spatial direct parthood.</rdfs:comment>
        <owl:versionInfo>In EMMO version 1.0.0-alpha2, physical quantities used the hasReferenceUnit object property to relate them to their units via physical dimensionality. This was simplified in 1.0.0-alpha3 in order to make reasoning faster.

The restriction (e.g. for the physical quantity Length)

    Length hasReferenceUnit only (hasPhysicsDimension only LengthDimension)

was in 1.0.0-alpha3 changed to

    Length hasPhysicsDimension some LengthDimension

Likewise were the universal restrictions on the corresponding unit changed to excistential. E.g.

    Metre hasPhysicsDimension only LengthDimension

was changed to

    Metre hasPhysicsDimension some LengthDimension

The label of this class was also changed from PhysicsDimension to PhysicalDimension.</owl:versionInfo>
        <skos:prefLabel xml:lang="en">hasReferenceUnit</skos:prefLabel>
    </owl:ObjectProperty>
    


    <!-- http://emmo.info/emmo/middle/metrology#EMMO_8ef3cd6d_ae58_4a8d_9fc0_ad8f49015cd0 -->

    <owl:ObjectProperty rdf:about="http://emmo.info/emmo/middle/metrology#EMMO_8ef3cd6d_ae58_4a8d_9fc0_ad8f49015cd0">
        <rdfs:subPropertyOf rdf:resource="http://emmo.info/emmo/middle/reductionistic#EMMO_b2282816_b7a3_44c6_b2cb_3feff1ceb7fe"/>
        <rdf:type rdf:resource="http://www.w3.org/2002/07/owl#InverseFunctionalProperty"/>
        <rdf:type rdf:resource="http://www.w3.org/2002/07/owl#AsymmetricProperty"/>
        <rdf:type rdf:resource="http://www.w3.org/2002/07/owl#IrreflexiveProperty"/>
        <rdfs:domain rdf:resource="http://emmo.info/emmo/middle/metrology#EMMO_f658c301_ce93_46cf_9639_4eace2c5d1d5"/>
        <rdfs:range rdf:resource="http://emmo.info/emmo/middle/math#EMMO_4ce76d7f_03f8_45b6_9003_90052a79bfaa"/>
        <rdfs:comment xml:lang="en">Relates a quantity to its reference unit through spatial direct parthood.</rdfs:comment>
        <skos:prefLabel xml:lang="en">hasQuantityValue</skos:prefLabel>
    </owl:ObjectProperty>
    


    <!-- http://emmo.info/emmo/middle/metrology#EMMO_bed1d005_b04e_4a90_94cf_02bc678a8569 -->

    <owl:ObjectProperty rdf:about="http://emmo.info/emmo/middle/metrology#EMMO_bed1d005_b04e_4a90_94cf_02bc678a8569">
        <rdfs:subPropertyOf rdf:resource="http://emmo.info/emmo/middle/properties#EMMO_e1097637_70d2_4895_973f_2396f04fa204"/>
        <rdfs:range rdf:resource="http://emmo.info/emmo/middle/metrology#EMMO_9895a1b4_f0a5_4167_ac5e_97db40b8bfcc"/>
        <skos:prefLabel xml:lang="en">hasPhysicalDimension</skos:prefLabel>
    </owl:ObjectProperty>
    


    <!-- 
    ///////////////////////////////////////////////////////////////////////////////////////
    //
    // Classes
    //
    ///////////////////////////////////////////////////////////////////////////////////////
     -->

    


    <!-- http://emmo.info/emmo/middle/metrology#EMMO_02c0621e_a527_4790_8a0f_2bb51973c819 -->

    <owl:Class rdf:about="http://emmo.info/emmo/middle/metrology#EMMO_02c0621e_a527_4790_8a0f_2bb51973c819">
        <rdfs:subClassOf rdf:resource="http://emmo.info/emmo/middle/math#EMMO_54ee6b5e_5261_44a8_86eb_5717e7fdb9d0"/>
        <rdfs:subClassOf>
            <owl:Restriction>
                <owl:onProperty rdf:resource="http://emmo.info/emmo/middle/metrology#EMMO_67fc0a36_8dcb_4ffa_9a43_31074efa3296"/>
                <owl:allValuesFrom rdf:resource="http://emmo.info/emmo/middle/metrology#EMMO_b081b346_7279_46ef_9a3d_2c088fcd79f4"/>
            </owl:Restriction>
        </rdfs:subClassOf>
        <owl:disjointUnionOf rdf:parseType="Collection">
            <rdf:Description rdf:about="http://emmo.info/emmo/middle/metrology#EMMO_71f6ab56_342c_484b_bbe0_de86b7367cb3"/>
            <rdf:Description rdf:about="http://emmo.info/emmo/middle/metrology#EMMO_acaaa124_3dde_48b6_86e6_6ec6f364f408"/>
        </owl:disjointUnionOf>
        <annotations:EMMO_967080e5_2f42_4eb2_a3a9_c58143e835f9 xml:lang="en">A &apos;Mathematical&apos; entity that is made of a &apos;Numeral&apos; and a &apos;MeasurementUnit&apos; defined by a physical law, connected to a physical entity through a model perspective. Measurement is done according to the same model.</annotations:EMMO_967080e5_2f42_4eb2_a3a9_c58143e835f9>
        <rdfs:comment xml:lang="en">In the same system of quantities, dim ρB = ML−3 is the quantity dimension of mass concentration of component B, and ML−3 is also the quantity dimension of mass density, ρ.
ISO 80000-1</rdfs:comment>
        <rdfs:comment xml:lang="en">Measured or simulated &apos;physical propertiy&apos;-s are always defined by a physical law, connected to a physical entity through a model perspective and measurement is done according to the same model.

Systems of units suggests that this is the correct approach, since except for the fundamental units (length, time, charge) every other unit is derived by mathematical relations between these fundamental units, implying a physical laws or definitions.</rdfs:comment>
        <rdfs:comment xml:lang="en">Measurement units of quantities of the same quantity dimension may be designated by the same name and symbol even when the quantities are not of the same kind. 

For example, joule per kelvin and J/K are respectively the name and symbol of both a measurement unit of heat capacity and a measurement unit of entropy, which are generally not considered to be quantities of the same kind. 

However, in some cases special measurement unit names are restricted to be used with quantities of specific kind only. 

For example, the measurement unit ‘second to the power minus one’ (1/s) is called hertz (Hz) when used for frequencies and becquerel (Bq) when used for activities of radionuclides. 

As another example, the joule (J) is used as a unit of energy, but never as a unit of moment of force, i.e. the newton metre (N · m).</rdfs:comment>
        <rdfs:comment xml:lang="en">— quantities of the same kind have the same quantity dimension,
— quantities of different quantity dimensions are always of different kinds, and
— quantities having the same quantity dimension are not necessarily of the same kind.
ISO 80000-1</rdfs:comment>
        <skos:prefLabel xml:lang="en">PhysicalQuantity</skos:prefLabel>
    </owl:Class>
    


    <!-- http://emmo.info/emmo/middle/metrology#EMMO_08b308d4_31cd_4779_a784_aa92fc730f39 -->

    <owl:Class rdf:about="http://emmo.info/emmo/middle/metrology#EMMO_08b308d4_31cd_4779_a784_aa92fc730f39">
        <annotations:EMMO_967080e5_2f42_4eb2_a3a9_c58143e835f9 xml:lang="en">Derived units are defined as products of powers of the base units corresponding to the relations defining the derived quantities in terms of the base quantities.</annotations:EMMO_967080e5_2f42_4eb2_a3a9_c58143e835f9>
        <skos:prefLabel xml:lang="en">DerivedUnit</skos:prefLabel>
    </owl:Class>
    


    <!-- http://emmo.info/emmo/middle/metrology#EMMO_0a318776_b067_4de0_a2a6_cba2cf6333f8 -->

    <owl:Class rdf:about="http://emmo.info/emmo/middle/metrology#EMMO_0a318776_b067_4de0_a2a6_cba2cf6333f8">
        <owl:equivalentClass>
            <owl:Class>
                <owl:intersectionOf rdf:parseType="Collection">
                    <rdf:Description rdf:about="http://emmo.info/emmo/middle/perceptual#EMMO_48716718_225f_4c88_89e2_d819d30c90a2"/>
                    <rdf:Description rdf:about="http://emmo.info/emmo/middle/perceptual#EMMO_a1083d0a_c1fb_471f_8e20_a98f881ad527"/>
                </owl:intersectionOf>
            </owl:Class>
        </owl:equivalentClass>
        <skos:prefLabel xml:lang="en">IdiomaticSymbol</skos:prefLabel>
    </owl:Class>
    


    <!-- http://emmo.info/emmo/middle/metrology#EMMO_18ce5200_00f5_45bb_8c6f_6fb128cd41ae -->

    <owl:Class rdf:about="http://emmo.info/emmo/middle/metrology#EMMO_18ce5200_00f5_45bb_8c6f_6fb128cd41ae">
        <rdfs:subClassOf rdf:resource="http://emmo.info/emmo/middle/metrology#EMMO_985bec21_989f_4b9e_a4b3_735d88099c3c"/>
        <rdfs:comment xml:lang="en">A reference can be a measurement unit, a measurement procedure, a reference material, or a combination of such.
International vocabulary of metrology (VIM)</rdfs:comment>
        <rdfs:comment xml:lang="en">A symbolic is recognized as reference unit also if it is not part of a quatity (e.g. as in the sentence &quot;the Bq is the reference unit of Becquerel&quot;).

For this reason we can&apos;t declare the axiom:
ReferenceUnit SubClassOf: inverse(hasReferenceUnit) some Quantity
because there exist reference units without being part of a quantity.

This is peculiar to EMMO, where quantities (symbolic) are distinct with properties (semiotics).</rdfs:comment>
        <skos:prefLabel xml:lang="en">ReferenceUnit</skos:prefLabel>
    </owl:Class>
    


    <!-- http://emmo.info/emmo/middle/metrology#EMMO_216f448e_cdbc_4aeb_a529_7a5fe7fc38bb -->

    <owl:Class rdf:about="http://emmo.info/emmo/middle/metrology#EMMO_216f448e_cdbc_4aeb_a529_7a5fe7fc38bb">
        <owl:equivalentClass>
            <owl:Class>
                <owl:intersectionOf rdf:parseType="Collection">
                    <rdf:Description rdf:about="http://emmo.info/emmo/middle/metrology#EMMO_b081b346_7279_46ef_9a3d_2c088fcd79f4"/>
                    <rdf:Description rdf:about="http://emmo.info/emmo/middle/perceptual#EMMO_a1083d0a_c1fb_471f_8e20_a98f881ad527"/>
                </owl:intersectionOf>
            </owl:Class>
        </owl:equivalentClass>
        <owl:disjointUnionOf rdf:parseType="Collection">
            <rdf:Description rdf:about="http://emmo.info/emmo/middle/metrology#EMMO_3ee80521_3c23_4dd1_935d_9d522614a3e2"/>
            <rdf:Description rdf:about="http://emmo.info/emmo/middle/metrology#EMMO_db716151_6b73_45ff_910c_d182fdcbb4f5"/>
        </owl:disjointUnionOf>
        <annotations:EMMO_967080e5_2f42_4eb2_a3a9_c58143e835f9 xml:lang="en">A symbol that stands for a single unit.</annotations:EMMO_967080e5_2f42_4eb2_a3a9_c58143e835f9>
        <annotations:EMMO_b432d2d5_25f4_4165_99c5_5935a7763c1a xml:lang="en">Some examples are &quot;Pa&quot;, &quot;m&quot; and &quot;J&quot;.</annotations:EMMO_b432d2d5_25f4_4165_99c5_5935a7763c1a>
        <skos:prefLabel xml:lang="en">UnitSymbol</skos:prefLabel>
    </owl:Class>
    


    <!-- http://emmo.info/emmo/middle/metrology#EMMO_3227b821_26a5_4c7c_9c01_5c24483e0bd0 -->

    <owl:Class rdf:about="http://emmo.info/emmo/middle/metrology#EMMO_3227b821_26a5_4c7c_9c01_5c24483e0bd0">
        <owl:equivalentClass>
            <owl:Restriction>
                <owl:onProperty rdf:resource="http://emmo.info/emmo/middle/perceptual#EMMO_23b579e1_8088_45b5_9975_064014026c42"/>
                <owl:hasValue>T0 L0 M0 I0 Θ0 N0 J0</owl:hasValue>
            </owl:Restriction>
        </owl:equivalentClass>
        <rdfs:subClassOf rdf:resource="http://emmo.info/emmo/middle/metrology#EMMO_9895a1b4_f0a5_4167_ac5e_97db40b8bfcc"/>
        <rdfs:comment xml:lang="en">&quot;The unit one is the neutral element of any system of units – necessary and present automatically.&quot;
SI Brochure</rdfs:comment>
        <skos:prefLabel xml:lang="en">DimensionOne</skos:prefLabel>
    </owl:Class>
    


    <!-- http://emmo.info/emmo/middle/metrology#EMMO_3ee80521_3c23_4dd1_935d_9d522614a3e2 -->

    <owl:Class rdf:about="http://emmo.info/emmo/middle/metrology#EMMO_3ee80521_3c23_4dd1_935d_9d522614a3e2">
        <rdfs:subClassOf rdf:resource="http://emmo.info/emmo/middle/metrology#EMMO_08b308d4_31cd_4779_a784_aa92fc730f39"/>
        <rdfs:subClassOf>
            <owl:Restriction>
                <owl:onProperty>
                    <rdf:Description>
                        <owl:inverseOf rdf:resource="http://emmo.info/emmo/middle/semiotics#EMMO_60577dea_9019_4537_ac41_80b0fb563d41"/>
                    </rdf:Description>
                </owl:onProperty>
                <owl:someValuesFrom rdf:resource="http://emmo.info/emmo/middle/metrology#EMMO_08b308d4_31cd_4779_a784_aa92fc730f39"/>
            </owl:Restriction>
        </rdfs:subClassOf>
        <annotations:EMMO_967080e5_2f42_4eb2_a3a9_c58143e835f9 xml:lang="en">A unit symbol that stands for a derived unit.</annotations:EMMO_967080e5_2f42_4eb2_a3a9_c58143e835f9>
        <annotations:EMMO_b432d2d5_25f4_4165_99c5_5935a7763c1a xml:lang="en">Pa stands for N/m2
J stands for N m</annotations:EMMO_b432d2d5_25f4_4165_99c5_5935a7763c1a>
        <rdfs:comment xml:lang="en">Special units are semiotic shortcuts to more complex composed symbolic objects.</rdfs:comment>
        <skos:prefLabel xml:lang="en">SpecialUnit</skos:prefLabel>
    </owl:Class>
    


    <!-- http://emmo.info/emmo/middle/metrology#EMMO_3f15d200_c97b_42c8_8ac0_d81d150361e2 -->

    <owl:Class rdf:about="http://emmo.info/emmo/middle/metrology#EMMO_3f15d200_c97b_42c8_8ac0_d81d150361e2">
        <annotations:EMMO_967080e5_2f42_4eb2_a3a9_c58143e835f9 xml:lang="en">For a given unit system, measured constants are physical constants that are not used to define the unit system. Hence, these constants have to be measured and will therefore be associated with an uncertainty.</annotations:EMMO_967080e5_2f42_4eb2_a3a9_c58143e835f9>
        <skos:prefLabel xml:lang="en">MeasuredConstant</skos:prefLabel>
    </owl:Class>
    


    <!-- http://emmo.info/emmo/middle/metrology#EMMO_50a3552e_859a_4ff7_946d_76d537cabce6 -->

    <owl:Class rdf:about="http://emmo.info/emmo/middle/metrology#EMMO_50a3552e_859a_4ff7_946d_76d537cabce6">
        <owl:equivalentClass>
            <owl:Class>
                <owl:intersectionOf rdf:parseType="Collection">
                    <rdf:Description rdf:about="http://emmo.info/emmo/middle/metrology#EMMO_985bec21_989f_4b9e_a4b3_735d88099c3c"/>
                    <rdf:Description rdf:about="http://emmo.info/emmo/middle/perceptual#EMMO_a1083d0a_c1fb_471f_8e20_a98f881ad527"/>
                </owl:intersectionOf>
            </owl:Class>
        </owl:equivalentClass>
        <rdfs:subClassOf>
            <owl:Restriction>
                <owl:onProperty rdf:resource="http://emmo.info/emmo/top/mereotopology#EMMO_9380ab64_0363_4804_b13f_3a8a94119a76"/>
                <owl:allValuesFrom>
                    <owl:Class>
                        <owl:complementOf rdf:resource="http://emmo.info/emmo/middle/metrology#EMMO_985bec21_989f_4b9e_a4b3_735d88099c3c"/>
                    </owl:Class>
                </owl:allValuesFrom>
            </owl:Restriction>
        </rdfs:subClassOf>
        <annotations:EMMO_967080e5_2f42_4eb2_a3a9_c58143e835f9 xml:lang="en">A symbol that stands for a concept in the language of the meterological domain of ISO 80000.</annotations:EMMO_967080e5_2f42_4eb2_a3a9_c58143e835f9>
        <skos:prefLabel xml:lang="en">MetrologicalSymbol</skos:prefLabel>
    </owl:Class>
    


    <!-- http://emmo.info/emmo/middle/metrology#EMMO_591e02fd_8d37_45a6_9d11_bb21cef391a0 -->

    <owl:Class rdf:about="http://emmo.info/emmo/middle/metrology#EMMO_591e02fd_8d37_45a6_9d11_bb21cef391a0">
        <rdfs:subClassOf rdf:resource="http://emmo.info/emmo/middle/metrology#EMMO_b081b346_7279_46ef_9a3d_2c088fcd79f4"/>
        <annotations:EMMO_967080e5_2f42_4eb2_a3a9_c58143e835f9 xml:lang="en">A unit that does not belong to any system of units.</annotations:EMMO_967080e5_2f42_4eb2_a3a9_c58143e835f9>
        <annotations:EMMO_b432d2d5_25f4_4165_99c5_5935a7763c1a xml:lang="en">eV
barn</annotations:EMMO_b432d2d5_25f4_4165_99c5_5935a7763c1a>
        <skos:prefLabel xml:lang="en">OffSystemUnit</skos:prefLabel>
    </owl:Class>
    


    <!-- http://emmo.info/emmo/middle/metrology#EMMO_5ebd5e01_0ed3_49a2_a30d_cd05cbe72978 -->

    <owl:Class rdf:about="http://emmo.info/emmo/middle/metrology#EMMO_5ebd5e01_0ed3_49a2_a30d_cd05cbe72978">
        <rdfs:subClassOf rdf:resource="http://emmo.info/emmo/middle/metrology#EMMO_08b308d4_31cd_4779_a784_aa92fc730f39"/>
        <rdfs:subClassOf>
            <owl:Restriction>
                <owl:onProperty rdf:resource="http://emmo.info/emmo/middle/metrology#EMMO_bed1d005_b04e_4a90_94cf_02bc678a8569"/>
                <owl:someValuesFrom rdf:resource="http://emmo.info/emmo/middle/metrology#EMMO_3227b821_26a5_4c7c_9c01_5c24483e0bd0"/>
            </owl:Restriction>
        </rdfs:subClassOf>
        <annotations:EMMO_1f1b164d_ec6a_4faa_8d5e_88bda62316cc>http://qudt.org/vocab/unit/UNITLESS</annotations:EMMO_1f1b164d_ec6a_4faa_8d5e_88bda62316cc>
        <annotations:EMMO_967080e5_2f42_4eb2_a3a9_c58143e835f9 xml:lang="en">Represents the number 1, used as an explicit unit to say something has no units.</annotations:EMMO_967080e5_2f42_4eb2_a3a9_c58143e835f9>
        <annotations:EMMO_b432d2d5_25f4_4165_99c5_5935a7763c1a xml:lang="en">Refractive index or volume fraction.</annotations:EMMO_b432d2d5_25f4_4165_99c5_5935a7763c1a>
        <annotations:EMMO_b432d2d5_25f4_4165_99c5_5935a7763c1a xml:lang="en">Typically used for ratios of two units whos dimensions cancels out.</annotations:EMMO_b432d2d5_25f4_4165_99c5_5935a7763c1a>
        <skos:prefLabel xml:lang="en">UnitOne</skos:prefLabel>
    </owl:Class>
    


    <!-- http://emmo.info/emmo/middle/metrology#EMMO_62f0d847_3603_45b4_bfc4_dd4511355ff2 -->

    <owl:Class rdf:about="http://emmo.info/emmo/middle/metrology#EMMO_62f0d847_3603_45b4_bfc4_dd4511355ff2">
        <annotations:EMMO_967080e5_2f42_4eb2_a3a9_c58143e835f9 xml:lang="en">Measurement unit obtained by multiplying a given measurement unit by an integer greater than one.</annotations:EMMO_967080e5_2f42_4eb2_a3a9_c58143e835f9>
        <skos:prefLabel xml:lang="en">MultipleUnit</skos:prefLabel>
    </owl:Class>
    


    <!-- http://emmo.info/emmo/middle/metrology#EMMO_71f6ab56_342c_484b_bbe0_de86b7367cb3 -->

    <owl:Class rdf:about="http://emmo.info/emmo/middle/metrology#EMMO_71f6ab56_342c_484b_bbe0_de86b7367cb3">
        <annotations:EMMO_967080e5_2f42_4eb2_a3a9_c58143e835f9 xml:lang="en">&quot;Quantity, in a system of quantities, defined in terms of the base quantities of that system&quot;.</annotations:EMMO_967080e5_2f42_4eb2_a3a9_c58143e835f9>
        <skos:prefLabel xml:lang="en">DerivedQuantity</skos:prefLabel>
    </owl:Class>
    


    <!-- http://emmo.info/emmo/middle/metrology#EMMO_7d2afa66_ae9e_4095_a9bf_421d0be401b6 -->

    <owl:Class rdf:about="http://emmo.info/emmo/middle/metrology#EMMO_7d2afa66_ae9e_4095_a9bf_421d0be401b6">
        <rdfs:subClassOf rdf:resource="http://emmo.info/emmo/middle/math#EMMO_ae15fb4f_8e4d_41de_a0f9_3997f89ba6a2"/>
        <rdfs:subClassOf rdf:resource="http://emmo.info/emmo/middle/metrology#EMMO_985bec21_989f_4b9e_a4b3_735d88099c3c"/>
        <rdfs:subClassOf rdf:resource="http://emmo.info/emmo/middle/perceptual#EMMO_a1083d0a_c1fb_471f_8e20_a98f881ad527"/>
        <annotations:EMMO_967080e5_2f42_4eb2_a3a9_c58143e835f9 xml:lang="en">Dimensionless multiplicative unit prefix.</annotations:EMMO_967080e5_2f42_4eb2_a3a9_c58143e835f9>
        <rdfs:seeAlso>https://en.wikipedia.org/wiki/Metric_prefix</rdfs:seeAlso>
        <skos:prefLabel xml:lang="en">MetricPrefix</skos:prefLabel>
    </owl:Class>
    


    <!-- http://emmo.info/emmo/middle/metrology#EMMO_868ae137_4d25_493e_b270_21ea3d94849e -->

    <owl:Class rdf:about="http://emmo.info/emmo/middle/metrology#EMMO_868ae137_4d25_493e_b270_21ea3d94849e">
        <owl:equivalentClass>
            <owl:Class>
                <owl:unionOf rdf:parseType="Collection">
                    <rdf:Description rdf:about="http://emmo.info/emmo/middle/metrology#EMMO_08b308d4_31cd_4779_a784_aa92fc730f39"/>
                    <rdf:Description rdf:about="http://emmo.info/emmo/middle/metrology#EMMO_216f448e_cdbc_4aeb_a529_7a5fe7fc38bb"/>
                </owl:unionOf>
            </owl:Class>
        </owl:equivalentClass>
        <rdfs:subClassOf>
            <owl:Restriction>
                <owl:onProperty rdf:resource="http://emmo.info/emmo/middle/reductionistic#EMMO_b2282816_b7a3_44c6_b2cb_3feff1ceb7fe"/>
                <owl:allValuesFrom>
                    <owl:Class>
                        <owl:complementOf rdf:resource="http://emmo.info/emmo/middle/metrology#EMMO_7d2afa66_ae9e_4095_a9bf_421d0be401b6"/>
                    </owl:Class>
                </owl:allValuesFrom>
            </owl:Restriction>
        </rdfs:subClassOf>
        <annotations:EMMO_967080e5_2f42_4eb2_a3a9_c58143e835f9 xml:lang="en">A measurement unit symbol that do not have a metric prefix as a direct spatial part.</annotations:EMMO_967080e5_2f42_4eb2_a3a9_c58143e835f9>
        <skos:prefLabel xml:lang="en">NonPrefixedUnit</skos:prefLabel>
    </owl:Class>
    


    <!-- http://emmo.info/emmo/middle/metrology#EMMO_89762966_8076_4f7c_b745_f718d653e8e2 -->

    <owl:Class rdf:about="http://emmo.info/emmo/middle/metrology#EMMO_89762966_8076_4f7c_b745_f718d653e8e2">
        <rdfs:comment xml:lang="en">Physical constant used to define a unit system. Hence, when expressed in that unit system they have an exact value with no associated uncertainty.</rdfs:comment>
        <skos:prefLabel xml:lang="en">ExactConstant</skos:prefLabel>
    </owl:Class>
    


    <!-- http://emmo.info/emmo/middle/metrology#EMMO_985bec21_989f_4b9e_a4b3_735d88099c3c -->

    <owl:Class rdf:about="http://emmo.info/emmo/middle/metrology#EMMO_985bec21_989f_4b9e_a4b3_735d88099c3c">
        <rdfs:subClassOf rdf:resource="http://emmo.info/emmo/middle/perceptual#EMMO_d8d2144e_5c8d_455d_a643_5caf4d8d9df8"/>
        <annotations:EMMO_967080e5_2f42_4eb2_a3a9_c58143e835f9 xml:lang="en">A language object used in metrology.</annotations:EMMO_967080e5_2f42_4eb2_a3a9_c58143e835f9>
        <rdfs:comment xml:lang="en">Metrology includes all theoretical and practical aspects of measurement, whatever the measurement uncertainty and field of application.

-- International vocabulary of metrology (VIM)</rdfs:comment>
        <rdfs:comment xml:lang="en">This language domain makes use of ISO 80000 concepts.</rdfs:comment>
        <skos:prefLabel xml:lang="en">Metrological</skos:prefLabel>
    </owl:Class>
    


    <!-- http://emmo.info/emmo/middle/metrology#EMMO_9895a1b4_f0a5_4167_ac5e_97db40b8bfcc -->

    <owl:Class rdf:about="http://emmo.info/emmo/middle/metrology#EMMO_9895a1b4_f0a5_4167_ac5e_97db40b8bfcc">
        <rdfs:subClassOf rdf:resource="http://emmo.info/emmo/middle/metrology#EMMO_985bec21_989f_4b9e_a4b3_735d88099c3c"/>
        <rdfs:subClassOf rdf:resource="http://emmo.info/emmo/middle/perceptual#EMMO_a1083d0a_c1fb_471f_8e20_a98f881ad527"/>
        <annotations:EMMO_967080e5_2f42_4eb2_a3a9_c58143e835f9 xml:lang="en">A symbol that, following SI specifications, describe the physical dimensionality of a physical quantity and the exponents of the base units in a measurement unit.</annotations:EMMO_967080e5_2f42_4eb2_a3a9_c58143e835f9>
        <rdfs:comment xml:lang="en">All physical quantities, with the exception of counts, are derived quantities, which may be written in terms of base quantities according to the equations of physics. The dimensions of the derived quantities are written as products of powers of the dimensions of the base quantities using the equations that relate the derived quantities to the base quantities.
In general the dimension of any quantity Q is written in the form of a dimensional product,

dim Q = T^α L^β M^γ I^δ Θ^ε N^ζ J^η

where the exponents α, β, γ, δ, ε, ζ and η, which are generally small integers, which can be positive, negative, or zero, are called the dimensional exponents.
(SI brochure)</rdfs:comment>
        <rdfs:comment xml:lang="en">The conventional symbolic representation of the dimension of a base quantity is a single upper case letter in roman (upright) type. The conventional symbolic representation of the dimension of a derived quantity is the product of powers of the dimensions of the base quantities according to the definition of the derived quantity. The dimension of a quantity Q is denoted by dim Q.
ISO 80000-1</rdfs:comment>
        <rdfs:comment xml:lang="en">The expression used by the EMMO for physical dimensions is a metrological symbol (but a string at meta level, i.e. the ontologist level) like this:
 
Ta Lb Mc Id Θe Nf Jg

where a, b, c, d, e, f and g are 0 or signed integers.

Regex for the physical dimension symbol for the EMMO is:
^T([+-][1-9]|0) L([+-][1-9]|0) M([+-][1-9]|0) I([+-][1-9]|0) Θ([+-][1-9]|0) N([+-][1-9]|0) J([+-][1-9]|0)$

Examples of correspondance between base units and physical dimensions are:
mol -&gt; T0 L0 M0 I0 Θ0 N+1 J0
s -&gt; T+1 L0 M0 I0 Θ0 N0 J0
A/m2 -&gt; T0 L0 M-2 I+1 Θ0 N0 J0</rdfs:comment>
        <skos:prefLabel xml:lang="en">PhysicalDimension</skos:prefLabel>
    </owl:Class>
    


    <!-- http://emmo.info/emmo/middle/metrology#EMMO_a2f94f33_71fa_443c_a1fb_d1685fc537ec -->

    <owl:Class rdf:about="http://emmo.info/emmo/middle/metrology#EMMO_a2f94f33_71fa_443c_a1fb_d1685fc537ec">
        <annotations:EMMO_967080e5_2f42_4eb2_a3a9_c58143e835f9 xml:lang="en">Measurement unit obtained by dividing a given measurement unit by an integer greater than one.</annotations:EMMO_967080e5_2f42_4eb2_a3a9_c58143e835f9>
        <skos:prefLabel xml:lang="en">SubMultipleUnit</skos:prefLabel>
    </owl:Class>
    


    <!-- http://emmo.info/emmo/middle/metrology#EMMO_acaaa124_3dde_48b6_86e6_6ec6f364f408 -->

    <owl:Class rdf:about="http://emmo.info/emmo/middle/metrology#EMMO_acaaa124_3dde_48b6_86e6_6ec6f364f408">
        <rdfs:subClassOf>
            <owl:Restriction>
                <owl:onProperty rdf:resource="http://emmo.info/emmo/middle/metrology#EMMO_67fc0a36_8dcb_4ffa_9a43_31074efa3296"/>
                <owl:allValuesFrom rdf:resource="http://emmo.info/emmo/middle/metrology#EMMO_db716151_6b73_45ff_910c_d182fdcbb4f5"/>
            </owl:Restriction>
        </rdfs:subClassOf>
        <annotations:EMMO_967080e5_2f42_4eb2_a3a9_c58143e835f9 xml:lang="en">&quot;Quantity in a conventionally chosen subset of a given system of quantities, where no quantity in the subset can be expressed in terms of the other quantities within that subset&quot;
ISO 80000-1</annotations:EMMO_967080e5_2f42_4eb2_a3a9_c58143e835f9>
        <skos:prefLabel xml:lang="en">BaseQuantity</skos:prefLabel>
    </owl:Class>
    


    <!-- http://emmo.info/emmo/middle/metrology#EMMO_acd1a504_ca32_4f30_86ad_0b62cea5bc02 -->

    <owl:Class rdf:about="http://emmo.info/emmo/middle/metrology#EMMO_acd1a504_ca32_4f30_86ad_0b62cea5bc02">
        <rdfs:subClassOf rdf:resource="http://emmo.info/emmo/middle/metrology#EMMO_18ce5200_00f5_45bb_8c6f_6fb128cd41ae"/>
        <annotations:EMMO_967080e5_2f42_4eb2_a3a9_c58143e835f9 xml:lang="en">A reference unit provided by a reference material.
International vocabulary of metrology (VIM)</annotations:EMMO_967080e5_2f42_4eb2_a3a9_c58143e835f9>
        <annotations:EMMO_b432d2d5_25f4_4165_99c5_5935a7763c1a xml:lang="en">Arbitrary amount-of-substance concentration of lutropin in a given sample of plasma (WHO international standard 80/552): 5.0 International Unit/l</annotations:EMMO_b432d2d5_25f4_4165_99c5_5935a7763c1a>
        <skos:prefLabel xml:lang="en">StandardUnit</skos:prefLabel>
    </owl:Class>
    


    <!-- http://emmo.info/emmo/middle/metrology#EMMO_b081b346_7279_46ef_9a3d_2c088fcd79f4 -->

    <owl:Class rdf:about="http://emmo.info/emmo/middle/metrology#EMMO_b081b346_7279_46ef_9a3d_2c088fcd79f4">
        <rdfs:subClassOf rdf:resource="http://emmo.info/emmo/middle/metrology#EMMO_18ce5200_00f5_45bb_8c6f_6fb128cd41ae"/>
        <rdfs:subClassOf>
            <owl:Restriction>
                <owl:onProperty rdf:resource="http://emmo.info/emmo/middle/metrology#EMMO_bed1d005_b04e_4a90_94cf_02bc678a8569"/>
                <owl:qualifiedCardinality rdf:datatype="http://www.w3.org/2001/XMLSchema#nonNegativeInteger">1</owl:qualifiedCardinality>
                <owl:onClass rdf:resource="http://emmo.info/emmo/middle/metrology#EMMO_9895a1b4_f0a5_4167_ac5e_97db40b8bfcc"/>
            </owl:Restriction>
        </rdfs:subClassOf>
        <owl:disjointUnionOf rdf:parseType="Collection">
            <rdf:Description rdf:about="http://emmo.info/emmo/middle/metrology#EMMO_868ae137_4d25_493e_b270_21ea3d94849e"/>
            <rdf:Description rdf:about="http://emmo.info/emmo/middle/metrology#EMMO_c6d4a5e0_7e95_44df_a6db_84ee0a8bbc8e"/>
        </owl:disjointUnionOf>
        <annotations:EMMO_967080e5_2f42_4eb2_a3a9_c58143e835f9 xml:lang="en">A &apos;Quantity&apos; that stands for the standard reference magnitude of a specific class of measurement processes, defined and adopted by convention or by law.

The numerical quantity value of the &apos;MeasurementUnit&apos; is conventionally 1 and does not appear.

Quantitative measurement results are expressed as a multiple of the &apos;MeasurementUnit&apos;.</annotations:EMMO_967080e5_2f42_4eb2_a3a9_c58143e835f9>
        <rdfs:comment xml:lang="en">&quot;Real scalar quantity, defined and adopted by convention, with which any other quantity of the same kind can be compared to express the ratio of the second quantity to the first one as a number&quot;
ISO 80000-1</rdfs:comment>
        <rdfs:comment xml:lang="en">&quot;Unit symbols are mathematical entities and not abbreviations.&quot;

&quot;Symbols for units are treated as mathematical entities. In expressing the value of a quantity as the product of a numerical value and a unit, both the numerical value and the unit may be treated by the ordinary rules of algebra.&quot;

https://www.bipm.org/utils/common/pdf/si-brochure/SI-Brochure-9-EN.pdf</rdfs:comment>
        <rdfs:comment xml:lang="en">While the SI brochure treats &apos;MeasurementUnit&apos; as a &apos;PhysicalQuantity&apos;, in the EMMO this is not possible since the latter always has two direct parts, a &apos;Numerical&apos; and a &apos;MeasurementUnit&apos;, while the former a single &apos;Symbol&apos;.

SI distinguishes between a quantity (an abstract concept) and the quantity value (a number and a reference). The EMMO, following strict nominalism, considers a SI quantity as a SI quantity value, collapsing the two concepts into one: the &apos;Quantity&apos;.

So, for the EMMO the symbol &quot;kg&quot; is not a physical quantity but a &apos;MeasurementUnit&apos;, while the string &quot;1 kg&quot; is &apos;Physical Quantity&apos;.</rdfs:comment>
        <skos:prefLabel xml:lang="en">MeasurementUnit</skos:prefLabel>
    </owl:Class>
    


    <!-- http://emmo.info/emmo/middle/metrology#EMMO_b953f2b1_c8d1_4dd9_b630_d3ef6580c2bb -->

    <owl:Class rdf:about="http://emmo.info/emmo/middle/metrology#EMMO_b953f2b1_c8d1_4dd9_b630_d3ef6580c2bb">
        <rdfs:subClassOf rdf:resource="http://emmo.info/emmo/middle/metrology#EMMO_02c0621e_a527_4790_8a0f_2bb51973c819"/>
        <owl:disjointUnionOf rdf:parseType="Collection">
            <rdf:Description rdf:about="http://emmo.info/emmo/middle/metrology#EMMO_3f15d200_c97b_42c8_8ac0_d81d150361e2"/>
            <rdf:Description rdf:about="http://emmo.info/emmo/middle/metrology#EMMO_89762966_8076_4f7c_b745_f718d653e8e2"/>
        </owl:disjointUnionOf>
        <annotations:EMMO_c84c6752_6d64_48cc_9500_e54a3c34898d>https://en.wikipedia.org/wiki/List_of_physical_constants</annotations:EMMO_c84c6752_6d64_48cc_9500_e54a3c34898d>
        <rdfs:comment xml:lang="en">Physical constants are categorised into &quot;exact&quot; and measured constants. 

With &quot;exact&quot; constants, we refer to physical constants that have an exact numerical value after the revision of the SI system that was enforsed May 2019.</rdfs:comment>
        <skos:prefLabel xml:lang="en">PhysicalConstant</skos:prefLabel>
    </owl:Class>
    


    <!-- http://emmo.info/emmo/middle/metrology#EMMO_c46f091c_0420_4c1a_af30_0a2c8ebcf7d7 -->

    <owl:Class rdf:about="http://emmo.info/emmo/middle/metrology#EMMO_c46f091c_0420_4c1a_af30_0a2c8ebcf7d7">
        <annotations:EMMO_967080e5_2f42_4eb2_a3a9_c58143e835f9 xml:lang="en">&quot;Quantity, defined by a conventional measurement procedure, for which a total ordering relation can be established, according to magnitude, with other quantities of the same kind, but for which no algebraic operations among those quantities exist&quot;
International vocabulary of metrology (VIM)</annotations:EMMO_967080e5_2f42_4eb2_a3a9_c58143e835f9>
        <annotations:EMMO_b432d2d5_25f4_4165_99c5_5935a7763c1a xml:lang="en">Hardness
Resilience</annotations:EMMO_b432d2d5_25f4_4165_99c5_5935a7763c1a>
        <rdfs:comment xml:lang="en">&quot;Ordinal quantities, such as Rockwell C hardness, are usually not considered to be part of a system of quantities because they are related to other quantities through empirical relations only.&quot;
International vocabulary of metrology (VIM)</rdfs:comment>
        <skos:prefLabel xml:lang="en">OrdinalQuantity</skos:prefLabel>
    </owl:Class>
    


    <!-- http://emmo.info/emmo/middle/metrology#EMMO_c6d4a5e0_7e95_44df_a6db_84ee0a8bbc8e -->

    <owl:Class rdf:about="http://emmo.info/emmo/middle/metrology#EMMO_c6d4a5e0_7e95_44df_a6db_84ee0a8bbc8e">
        <rdfs:subClassOf>
            <owl:Restriction>
                <owl:onProperty rdf:resource="http://emmo.info/emmo/middle/reductionistic#EMMO_b2282816_b7a3_44c6_b2cb_3feff1ceb7fe"/>
                <owl:allValuesFrom>
                    <owl:Class>
                        <owl:unionOf rdf:parseType="Collection">
                            <rdf:Description rdf:about="http://emmo.info/emmo/middle/metrology#EMMO_216f448e_cdbc_4aeb_a529_7a5fe7fc38bb"/>
                            <rdf:Description rdf:about="http://emmo.info/emmo/middle/metrology#EMMO_7d2afa66_ae9e_4095_a9bf_421d0be401b6"/>
                        </owl:unionOf>
                    </owl:Class>
                </owl:allValuesFrom>
            </owl:Restriction>
        </rdfs:subClassOf>
        <rdfs:subClassOf>
            <owl:Restriction>
                <owl:onProperty rdf:resource="http://emmo.info/emmo/middle/reductionistic#EMMO_b2282816_b7a3_44c6_b2cb_3feff1ceb7fe"/>
                <owl:qualifiedCardinality rdf:datatype="http://www.w3.org/2001/XMLSchema#nonNegativeInteger">1</owl:qualifiedCardinality>
                <owl:onClass rdf:resource="http://emmo.info/emmo/middle/metrology#EMMO_216f448e_cdbc_4aeb_a529_7a5fe7fc38bb"/>
            </owl:Restriction>
        </rdfs:subClassOf>
        <rdfs:subClassOf>
            <owl:Restriction>
                <owl:onProperty rdf:resource="http://emmo.info/emmo/middle/reductionistic#EMMO_b2282816_b7a3_44c6_b2cb_3feff1ceb7fe"/>
                <owl:qualifiedCardinality rdf:datatype="http://www.w3.org/2001/XMLSchema#nonNegativeInteger">1</owl:qualifiedCardinality>
                <owl:onClass rdf:resource="http://emmo.info/emmo/middle/metrology#EMMO_7d2afa66_ae9e_4095_a9bf_421d0be401b6"/>
            </owl:Restriction>
        </rdfs:subClassOf>
        <owl:disjointUnionOf rdf:parseType="Collection">
            <rdf:Description rdf:about="http://emmo.info/emmo/middle/metrology#EMMO_62f0d847_3603_45b4_bfc4_dd4511355ff2"/>
            <rdf:Description rdf:about="http://emmo.info/emmo/middle/metrology#EMMO_a2f94f33_71fa_443c_a1fb_d1685fc537ec"/>
        </owl:disjointUnionOf>
        <annotations:EMMO_967080e5_2f42_4eb2_a3a9_c58143e835f9 xml:lang="en">A measurement unit that is made of a metric prefix and a unit symbol.</annotations:EMMO_967080e5_2f42_4eb2_a3a9_c58143e835f9>
        <skos:prefLabel xml:lang="en">PrefixedUnit</skos:prefLabel>
    </owl:Class>
    


    <!-- http://emmo.info/emmo/middle/metrology#EMMO_c9c8f824_9127_4f93_bc21_69fe78a7f6f2 -->

    <owl:Class rdf:about="http://emmo.info/emmo/middle/metrology#EMMO_c9c8f824_9127_4f93_bc21_69fe78a7f6f2">
        <rdfs:subClassOf rdf:resource="http://emmo.info/emmo/middle/metrology#EMMO_18ce5200_00f5_45bb_8c6f_6fb128cd41ae"/>
        <annotations:EMMO_967080e5_2f42_4eb2_a3a9_c58143e835f9 xml:lang="en">A reference unit provided by a measurement procedure.</annotations:EMMO_967080e5_2f42_4eb2_a3a9_c58143e835f9>
        <annotations:EMMO_b432d2d5_25f4_4165_99c5_5935a7763c1a xml:lang="en">Rockwell C hardness of a given sample (150 kg load): 43.5HRC(150 kg)</annotations:EMMO_b432d2d5_25f4_4165_99c5_5935a7763c1a>
        <skos:prefLabel xml:lang="en">ProcedureUnit</skos:prefLabel>
    </owl:Class>
    


    <!-- http://emmo.info/emmo/middle/metrology#EMMO_db716151_6b73_45ff_910c_d182fdcbb4f5 -->

    <owl:Class rdf:about="http://emmo.info/emmo/middle/metrology#EMMO_db716151_6b73_45ff_910c_d182fdcbb4f5">
        <annotations:EMMO_967080e5_2f42_4eb2_a3a9_c58143e835f9 xml:lang="en">A set of units that correspond to the base quantities in a system of units.</annotations:EMMO_967080e5_2f42_4eb2_a3a9_c58143e835f9>
        <skos:prefLabel xml:lang="en">BaseUnit</skos:prefLabel>
    </owl:Class>
    


    <!-- http://emmo.info/emmo/middle/metrology#EMMO_dd4a7f3e_ef56_466c_ac1a_d2716b5f87ec -->

    <owl:Class rdf:about="http://emmo.info/emmo/middle/metrology#EMMO_dd4a7f3e_ef56_466c_ac1a_d2716b5f87ec">
        <rdfs:subClassOf rdf:resource="http://emmo.info/emmo/middle/metrology#EMMO_f658c301_ce93_46cf_9639_4eace2c5d1d5"/>
    </owl:Class>
    


    <!-- http://emmo.info/emmo/middle/metrology#EMMO_f658c301_ce93_46cf_9639_4eace2c5d1d5 -->

    <owl:Class rdf:about="http://emmo.info/emmo/middle/metrology#EMMO_f658c301_ce93_46cf_9639_4eace2c5d1d5">
        <rdfs:subClassOf rdf:resource="http://emmo.info/emmo/middle/metrology#EMMO_985bec21_989f_4b9e_a4b3_735d88099c3c"/>
        <rdfs:subClassOf>
            <owl:Restriction>
                <owl:onProperty rdf:resource="http://emmo.info/emmo/middle/metrology#EMMO_67fc0a36_8dcb_4ffa_9a43_31074efa3296"/>
                <owl:qualifiedCardinality rdf:datatype="http://www.w3.org/2001/XMLSchema#nonNegativeInteger">1</owl:qualifiedCardinality>
                <owl:onClass rdf:resource="http://emmo.info/emmo/middle/metrology#EMMO_18ce5200_00f5_45bb_8c6f_6fb128cd41ae"/>
            </owl:Restriction>
        </rdfs:subClassOf>
        <rdfs:subClassOf>
            <owl:Restriction>
                <owl:onProperty rdf:resource="http://emmo.info/emmo/middle/metrology#EMMO_8ef3cd6d_ae58_4a8d_9fc0_ad8f49015cd0"/>
                <owl:qualifiedCardinality rdf:datatype="http://www.w3.org/2001/XMLSchema#nonNegativeInteger">1</owl:qualifiedCardinality>
                <owl:onClass rdf:resource="http://emmo.info/emmo/middle/math#EMMO_4ce76d7f_03f8_45b6_9003_90052a79bfaa"/>
            </owl:Restriction>
        </rdfs:subClassOf>
        <owl:disjointUnionOf rdf:parseType="Collection">
            <rdf:Description rdf:about="http://emmo.info/emmo/middle/metrology#EMMO_02c0621e_a527_4790_8a0f_2bb51973c819"/>
            <rdf:Description rdf:about="http://emmo.info/emmo/middle/metrology#EMMO_c46f091c_0420_4c1a_af30_0a2c8ebcf7d7"/>
        </owl:disjointUnionOf>
        <annotations:EMMO_967080e5_2f42_4eb2_a3a9_c58143e835f9 xml:lang="en">A symbolic that has parts a reference unit and a numerical object separated by a space expressing the value of a quantitative property (expressed as the product of the numerical and the unit).</annotations:EMMO_967080e5_2f42_4eb2_a3a9_c58143e835f9>
        <annotations:EMMO_b432d2d5_25f4_4165_99c5_5935a7763c1a xml:lang="en">6.8 m
0.9 km
8 K
6 MeV
43.5 HRC(150 kg)</annotations:EMMO_b432d2d5_25f4_4165_99c5_5935a7763c1a>
        <rdfs:comment xml:lang="en">A quantity is not necessarily a property, since it is possible to write &quot;10 kg&quot;, without assigning this quantity to a specific object.

However, a quantitative property is always a quantity.</rdfs:comment>
        <rdfs:comment xml:lang="en">Referred as Quantity Value in International vocabulary of metrology (VIM)</rdfs:comment>
        <rdfs:comment xml:lang="en">SI distinguishes between a quantity (an abstract concept) and the quantity value (a number and a reference). 

The EMMO, following strict nominalism, denies the existence of abstract objects and then collapses the two concepts of SI quantity and SI quantity value into a single one: the &apos;Quantity&apos;.

So, for the EMMO the symbol &quot;kg&quot; is not a physical quantity but simply a &apos;Symbolic&apos; object categorized as a &apos;MeasurementUnit&apos;.

While the string &quot;1 kg&quot; is a &apos;Physical Quantity&apos;.</rdfs:comment>
        <skos:prefLabel xml:lang="en">Quantity</skos:prefLabel>
    </owl:Class>
</rdf:RDF>



<!-- Generated by the OWL API (version 4.5.9.2019-02-01T07:24:44Z) https://github.com/owlcs/owlapi -->

