<?xml version="1.0"?>
<rdf:RDF xmlns="http://emmo.info/emmo/top/physical#"
     xml:base="http://emmo.info/emmo/top/physical"
     xmlns:owl="http://www.w3.org/2002/07/owl#"
     xmlns:rdf="http://www.w3.org/1999/02/22-rdf-syntax-ns#"
     xmlns:xml="http://www.w3.org/XML/1998/namespace"
     xmlns:xsd="http://www.w3.org/2001/XMLSchema#"
     xmlns:rdfs="http://www.w3.org/2000/01/rdf-schema#"
     xmlns:skos="http://www.w3.org/2004/02/skos/core#"
     xmlns:dcterms="http://purl.org/dc/terms/"
     xmlns:annotations="http://emmo.info/emmo/top/annotations#">
    <owl:Ontology rdf:about="http://emmo.info/emmo/top/physical">
        <owl:versionIRI rdf:resource="http://emmo.info/emmo/1.0.0-alpha2/top/physical"/>
        <owl:imports rdf:resource="http://emmo.info/emmo/1.0.0-alpha2/top/mereotopology"/>
        <dcterms:abstract xml:lang="en">European Materials &amp; Modelling Ontology (EMMO)

EMMO is a multidisciplinary effort to develop a standard representational framework (the ontology) based on current materials modelling knowledge, including physical sciences, analytical philosophy and information and communication technologies.

It provides the connection between the physical world, materials characterisation world and materials modelling world.

EMMO is released under a Creative Commons license Attribution 4.0 International (CC BY 4.0).</dcterms:abstract>
        <dcterms:contributor>Access, DE</dcterms:contributor>
        <dcterms:contributor>Fraunhofer IWM, DE</dcterms:contributor>
        <dcterms:contributor>Goldbeck Consulting Ltd (UK)</dcterms:contributor>
        <dcterms:contributor>SINTEF, NO</dcterms:contributor>
        <dcterms:contributor>University of Bologna, IT</dcterms:contributor>
        <dcterms:creator>Adham Hashibon</dcterms:creator>
        <dcterms:creator>Emanuele Ghedini</dcterms:creator>
        <dcterms:creator>Georg Schmitz</dcterms:creator>
        <dcterms:creator>Gerhard Goldbeck</dcterms:creator>
        <dcterms:creator>Jesper Friis</dcterms:creator>
        <dcterms:license>https://creativecommons.org/licenses/by/4.0/legalcode</dcterms:license>
        <dcterms:publisher>EMMC ASBL</dcterms:publisher>
        <dcterms:title xml:lang="en">European Materials &amp; Modelling Ontology</dcterms:title>
        <rdfs:comment xml:lang="en">Contacts:
Gerhard Goldbeck
Goldbeck Consulting Ltd (UK)
email: gerhard@goldbeck-consulting.com

Emanuele Ghedini
University of Bologna (IT)
email: emanuele.ghedini@unibo.it</rdfs:comment>
        <rdfs:comment xml:lang="en">The EMMO requires FacT++ reasoner plugin in order to visualize all inferences and class hierarchy (ctrl+R hotkey in Protege).</rdfs:comment>
        <owl:versionInfo>1.0.0-alpha2</owl:versionInfo>
    </owl:Ontology>
    


    <!-- 
    ///////////////////////////////////////////////////////////////////////////////////////
    //
    // Object Properties
    //
    ///////////////////////////////////////////////////////////////////////////////////////
     -->

    


    <!-- http://emmo.info/emmo/top/physical#EMMO_6e046dd0_9634_4013_b2b1_9cc468087c83 -->

    <owl:ObjectProperty rdf:about="http://emmo.info/emmo/top/physical#EMMO_6e046dd0_9634_4013_b2b1_9cc468087c83">
        <rdfs:subPropertyOf rdf:resource="http://emmo.info/emmo/top/mereotopology#EMMO_9380ab64_0363_4804_b13f_3a8a94119a76"/>
        <rdf:type rdf:resource="http://www.w3.org/2002/07/owl#TransitiveProperty"/>
        <rdfs:domain rdf:resource="http://emmo.info/emmo/top/mereotopology#EMMO_eb3a768e_d53e_4be9_a23b_0714833c36de"/>
        <rdfs:range rdf:resource="http://emmo.info/emmo/top/mereotopology#EMMO_eb3a768e_d53e_4be9_a23b_0714833c36de"/>
        <annotations:EMMO_967080e5_2f42_4eb2_a3a9_c58143e835f9>A relation that isolates a proper part that extends itself in time through a portion of the lifetime whole.</annotations:EMMO_967080e5_2f42_4eb2_a3a9_c58143e835f9>
        <skos:prefLabel xml:lang="en">hasSpatioTemporalPart</skos:prefLabel>
    </owl:ObjectProperty>
    


    <!-- http://emmo.info/emmo/top/physical#EMMO_7afbed84_7593_4a23_bd88_9d9c6b04e8f6 -->

    <owl:ObjectProperty rdf:about="http://emmo.info/emmo/top/physical#EMMO_7afbed84_7593_4a23_bd88_9d9c6b04e8f6">
        <rdfs:subPropertyOf rdf:resource="http://emmo.info/emmo/top/mereotopology#EMMO_9380ab64_0363_4804_b13f_3a8a94119a76"/>
        <rdf:type rdf:resource="http://www.w3.org/2002/07/owl#TransitiveProperty"/>
        <rdfs:domain rdf:resource="http://emmo.info/emmo/top/mereotopology#EMMO_eb3a768e_d53e_4be9_a23b_0714833c36de"/>
        <rdfs:range rdf:resource="http://emmo.info/emmo/top/mereotopology#EMMO_eb3a768e_d53e_4be9_a23b_0714833c36de"/>
        <annotations:EMMO_967080e5_2f42_4eb2_a3a9_c58143e835f9>A relation that isolate a proper part that covers the total spatial extension of a whole within a time interval.</annotations:EMMO_967080e5_2f42_4eb2_a3a9_c58143e835f9>
        <skos:prefLabel xml:lang="en">hasTemporalPart</skos:prefLabel>
    </owl:ObjectProperty>
    


    <!-- http://emmo.info/emmo/top/physical#EMMO_f68030be_94b8_4c61_a161_886468558054 -->

    <owl:ObjectProperty rdf:about="http://emmo.info/emmo/top/physical#EMMO_f68030be_94b8_4c61_a161_886468558054">
        <rdfs:subPropertyOf rdf:resource="http://emmo.info/emmo/top/mereotopology#EMMO_9380ab64_0363_4804_b13f_3a8a94119a76"/>
        <rdf:type rdf:resource="http://www.w3.org/2002/07/owl#TransitiveProperty"/>
        <rdfs:domain rdf:resource="http://emmo.info/emmo/top/mereotopology#EMMO_eb3a768e_d53e_4be9_a23b_0714833c36de"/>
        <rdfs:range rdf:resource="http://emmo.info/emmo/top/mereotopology#EMMO_eb3a768e_d53e_4be9_a23b_0714833c36de"/>
        <annotations:EMMO_967080e5_2f42_4eb2_a3a9_c58143e835f9>A relation that isolates a proper part that extends itself in time within the overall lifetime of the whole, without covering the full spatial extension of the 4D whole (i.e. is not a temporal part).</annotations:EMMO_967080e5_2f42_4eb2_a3a9_c58143e835f9>
        <skos:prefLabel xml:lang="en">hasSpatialPart</skos:prefLabel>
    </owl:ObjectProperty>
    


    <!-- 
    ///////////////////////////////////////////////////////////////////////////////////////
    //
    // Classes
    //
    ///////////////////////////////////////////////////////////////////////////////////////
     -->

    


    <!-- http://emmo.info/emmo/top/mereotopology#EMMO_eb3a768e_d53e_4be9_a23b_0714833c36de -->

    <owl:Class rdf:about="http://emmo.info/emmo/top/mereotopology#EMMO_eb3a768e_d53e_4be9_a23b_0714833c36de">
        <owl:disjointUnionOf rdf:parseType="Collection">
            <rdf:Description rdf:about="http://emmo.info/emmo/top/physical#EMMO_29072ec4_ffcb_42fb_bdc7_26f05a2e9873"/>
            <rdf:Description rdf:about="http://emmo.info/emmo/top/physical#EMMO_c5ddfdba_c074_4aa4_ad6b_1ac4942d300d"/>
        </owl:disjointUnionOf>
    </owl:Class>
    


    <!-- http://emmo.info/emmo/top/physical#EMMO_0f795e3e_c602_4577_9a43_d5a231aa1360 -->

    <owl:Class rdf:about="http://emmo.info/emmo/top/physical#EMMO_0f795e3e_c602_4577_9a43_d5a231aa1360">
        <rdfs:subClassOf rdf:resource="http://emmo.info/emmo/top/physical#EMMO_c5ddfdba_c074_4aa4_ad6b_1ac4942d300d"/>
        <rdfs:subClassOf>
            <owl:Restriction>
                <owl:onProperty rdf:resource="http://emmo.info/emmo/top/physical#EMMO_7afbed84_7593_4a23_bd88_9d9c6b04e8f6"/>
                <owl:allValuesFrom rdf:resource="http://emmo.info/emmo/top/physical#EMMO_0f795e3e_c602_4577_9a43_d5a231aa1360"/>
            </owl:Restriction>
        </rdfs:subClassOf>
        <rdfs:subClassOf>
            <owl:Restriction>
                <owl:onProperty rdf:resource="http://emmo.info/emmo/top/physical#EMMO_f68030be_94b8_4c61_a161_886468558054"/>
                <owl:allValuesFrom rdf:resource="http://www.w3.org/2002/07/owl#Nothing"/>
            </owl:Restriction>
        </rdfs:subClassOf>
        <annotations:EMMO_967080e5_2f42_4eb2_a3a9_c58143e835f9 xml:lang="en">The basic constituent of &apos;item&apos;-s that can be proper partitioned only in time up to quantum level.</annotations:EMMO_967080e5_2f42_4eb2_a3a9_c58143e835f9>
        <rdfs:comment xml:lang="en">According to mereology, this should be call &apos;a-tomistic&apos; in the strict etimological sense of the word (from greek, a-tomos: un-divisible).

Mereology based on such items is called atomistic mereology.

However, in order not to confuse the lexicon between mereology and physics (in which an atom is a divisible physical entity) we prefer to call it &apos;elementary&apos;, recalling the concept of elementary particle coming from the standard particles model.</rdfs:comment>
        <rdfs:comment xml:lang="en">From Latin elementārius (“elementary”), from elementum (“one of the four elements of antiquity; fundamentals”)</rdfs:comment>
        <rdfs:comment xml:lang="en">While a &apos;Quantum&apos; is a-tomistic in time and space, an &apos;elementary&apos; is a-tomistic only in space, recalling the concept of elementary particle.</rdfs:comment>
        <skos:prefLabel xml:lang="en">Elementary</skos:prefLabel>
    </owl:Class>
    


    <!-- http://emmo.info/emmo/top/physical#EMMO_29072ec4_ffcb_42fb_bdc7_26f05a2e9873 -->

    <owl:Class rdf:about="http://emmo.info/emmo/top/physical#EMMO_29072ec4_ffcb_42fb_bdc7_26f05a2e9873">
        <rdfs:subClassOf>
            <owl:Restriction>
                <owl:onProperty rdf:resource="http://emmo.info/emmo/top/mereotopology#EMMO_17e27c22_37e1_468c_9dd7_95e137f73e7f"/>
                <owl:allValuesFrom rdf:resource="http://emmo.info/emmo/top/physical#EMMO_29072ec4_ffcb_42fb_bdc7_26f05a2e9873"/>
            </owl:Restriction>
        </rdfs:subClassOf>
        <annotations:EMMO_967080e5_2f42_4eb2_a3a9_c58143e835f9 xml:lang="en">A &apos;Item&apos; that has no &apos;Physical&apos; parts.</annotations:EMMO_967080e5_2f42_4eb2_a3a9_c58143e835f9>
        <rdfs:comment xml:lang="en">From Latin vacuus, “empty”.</rdfs:comment>
        <rdfs:comment xml:lang="en">The void concept is paramount for the representation of physical systems according to quantum theory.</rdfs:comment>
        <skos:prefLabel xml:lang="en">Void</skos:prefLabel>
    </owl:Class>
    


    <!-- http://emmo.info/emmo/top/physical#EMMO_c5ddfdba_c074_4aa4_ad6b_1ac4942d300d -->

    <owl:Class rdf:about="http://emmo.info/emmo/top/physical#EMMO_c5ddfdba_c074_4aa4_ad6b_1ac4942d300d">
        <rdfs:subClassOf>
            <owl:Restriction>
                <owl:onProperty rdf:resource="http://emmo.info/emmo/top/mereotopology#EMMO_17e27c22_37e1_468c_9dd7_95e137f73e7f"/>
                <owl:someValuesFrom rdf:resource="http://emmo.info/emmo/top/physical#EMMO_0f795e3e_c602_4577_9a43_d5a231aa1360"/>
            </owl:Restriction>
        </rdfs:subClassOf>
        <rdfs:subClassOf>
            <owl:Restriction>
                <owl:onProperty rdf:resource="http://emmo.info/emmo/top/physical#EMMO_7afbed84_7593_4a23_bd88_9d9c6b04e8f6"/>
                <owl:allValuesFrom rdf:resource="http://emmo.info/emmo/top/physical#EMMO_c5ddfdba_c074_4aa4_ad6b_1ac4942d300d"/>
            </owl:Restriction>
        </rdfs:subClassOf>
        <annotations:EMMO_967080e5_2f42_4eb2_a3a9_c58143e835f9 xml:lang="en">A &apos;Item&apos; that has part some &apos;Elementary&apos; and whose temporal proper parts are only &apos;Physical&apos;-s (i.e. it can be perceived without interruptions in time).</annotations:EMMO_967080e5_2f42_4eb2_a3a9_c58143e835f9>
        <rdfs:comment xml:lang="en">A &apos;Physical&apos; is the class that contains all the individuals that stand for real world objects that interact physically with the ontologist, i.e. physical objects.

A physical object must be perceived through physical interaction by the ontologist. Then the ontologist can declare an individual standing for the physical object just perceived.

Perception is a subcategory of physical interactions. It is an interaction that stimulate a representation of the physical object within the ontologist (the agent).</rdfs:comment>
        <rdfs:comment xml:lang="en">A &apos;Physical&apos; must include at least an &apos;Elementary&apos; part, and can include &apos;Void&apos; parts.

A &apos;Physical&apos; may include as part also the &apos;Void&apos; surrounding or enclosed by its &apos;Physical&apos; sub parts.

There are no particular criteria for &apos;Physical&apos;-s structure, except that is made of some &apos;Elementary&apos;-s as proper parts and not only &apos;Void&apos;.

This is done in order to take into account the quantum nature of physical systems, in which the actual position of sub-components (e.g. electrons in an atom) is not known except for its probability distribution function (according to the Copenhagen interpretation.)

e.g. a real world object that has spatial parts an atom and a cubic light year of void, extending for some time, can be a physical object.</rdfs:comment>
        <rdfs:comment xml:lang="en">A &apos;Physical&apos; with dimensions other than 4D cannot exist, following the restriction of the parent &apos;EMMO&apos; class.

It follows from the fact that perception is always unfolding in time.

e.g. you always have an aperture time when you take a picture or measure a property. Instantaneous perceptions are idealizations (abstractions) or a very small time measurement.</rdfs:comment>
        <rdfs:comment xml:lang="en">From Latin physica &quot;study of nature&quot; (and Ancient Greek φυσικός, “natural”). 

Here the word relates to things perceived through the senses as opposed to the mind; tangible or concrete.</rdfs:comment>
        <rdfs:comment xml:lang="en">In the EMMO there are no relations such as occupiesSpace, since &apos;Physical&apos;-s are themselves the 4D regions.</rdfs:comment>
        <rdfs:comment xml:lang="en">The EMMO can be used to represent real world entities as &apos;Physical&apos;-s that are easy to connect to classical or quantum mechanical based models.

Classical mechanics poses no representational issues, for the EMMO: the 4D representation of &apos;Physical&apos;-s is consistent with classical physics systems.

However, the representation of &apos;Physical&apos;-s that are typically analized through quantum mechanics (e.g. molecules, atoms, clusters), is not straightforward.

1) De Broglie - Bohm interpretation
The most simple approach is to rely on Bohmian mechanics, in which each particle is supposed to exists in a specific position between measurements (hidden variables approach), while its trajectory is calculated using a Guiding Equation based on a quantum field calculated with the Schroedinger Equation.

While this approach is really easy to implement in an ontology, since each entity has its own well defined 4D region, its mathematical representation failed to receive large consensus due to the difficulties to include relativistic effects, to be extended to subnuclear scale and the strong non-locality assumtpion of the quantum field.

Nevertheless, the Bohmian mechanics is a numerical approach that is used in electronic models to reduce the computational effort of the solution of Schroedinger Equation.

In practice, an EMMO user can declare a &apos;physical&apos; individual that stand for the whole quantum system to be described, and at the same time all sub-parts individuals can be declared, having them a well defined position in time, according to De Broglie - Bohm interpretation. The Hamiltonian can be calculated by considering the sub-part individuals.

&apos;physical&apos;-s are then made of &apos;physical&apos; parts and &apos;void&apos; parts that stand for the space between &apos;physical&apos;-s (e.g. the void between electrons and nucleus in an atom).

2) Copenhagen interpretation
In this interpretation the properties (e.g. energy level, position, spin) of a particle are not defined in the interval between two measurements and the quantum system is entangled (i.e. properties of particles in the sysyem are correlated) and described by a global wavefunction obtained solving the Schroedinger Equation. 

Upon measurement, the wavefunction collapses to a combination of close eigenstates that provide information about bservables of the system components (e.g. position, energy).

The EMMO can be used to represent &apos;physical&apos;-s that can be related to Copenhagen based models. In practice, the user should follow these steps:

a) define the quantum system as a &apos;physical&apos; individual (e.g. an H2 molecule) under a specific class (e.g. &apos;h2_molecule&apos;). This individual is the whole.

b) define the axioms of the  class that describe how many sub-parts are expected for the whole and their class types (e.g. &apos;h2_molecule&apos; has axioms &apos;has_proper_part exactly 2 electron&apos; and &apos;has_proper_part exactly 2 nucleus)

c) the user can now connect the whole to a Schroedinger equation based model whose Hamiltonian is calculated trough the information coming only from the axioms. No individuals are declared for the subparts!

d) a measurement done on the quantum system that provides information on the sub-part observables is interpreted as wavefunction collapse and leads to the end of the whole and the declaration of the sub-parts individuals which can be themselves other quantum systems 

e.g. if the outer electron of the H2 molecule interacts with another entity defining its state, then the whole that stands for the entangled H2 molecule becomes a &apos;physical&apos; made of an electron individual, a quantum system made of one electron and two nuclei and the void between them.

e.g. in the Born-Oppenheimer approximation the user represent the atom by un-entangling nucleus and electronic cloud. The un-entanglement comes in the form of declaration of individual as parts.

e.g. the double slit experiment can be represent in the EMMO as:
a) before the slit: a &apos;physical&apos; that extend in space and has parts &apos;electron&apos; and &apos;void&apos;, called &apos;single_electron_wave_function&apos;. &apos;electron&apos; and &apos;void&apos; are only in the axioms and not decalred individuals.
b) during slit passage: a &apos;physical&apos; made of one declared individual, the &apos;electron&apos;.
c) after the slit: again &apos;single_electron_wave_function&apos;
d) upon collision with the detector:  &apos;physical&apos; made of one declared individual, the &apos;electron&apos;.</rdfs:comment>
        <rdfs:comment xml:lang="en">The purpose of the &apos;Physical&apos; branch is to provide a representation of the real world objects, while the models used to name, explain or predict the behaviour of the real world objects lay under the &apos;Semiotic&apos; branch.

More than one semiotic representation can be connected to the same &apos;Physical&apos;.

e.g. Navier-Stokes or Euler equation applied to the same fluid are an example of mathematical model used to represent a physical object for some specific interpreter.</rdfs:comment>
        <skos:prefLabel xml:lang="en">Physical</skos:prefLabel>
    </owl:Class>
</rdf:RDF>



<!-- Generated by the OWL API (version 4.5.9.2019-02-01T07:24:44Z) https://github.com/owlcs/owlapi -->

